Some properties of locally closed terms were demonstrated, and well-defined lambda terms were defined.

Lambda/Basic.lean
@@ -7,12 +7,12 @@ inductive Lambda
 | app : Lambda → Lambda → Lambda
 deriving DecidableEq, Repr
 
-abbrev Λ := Lambda
+abbrev Λ' := Lambda
 
 prefix:100 "λ " => Lambda.abs
 prefix:100 "°" => Lambda.bvar
 
-def Lambda.toString : Λ → String
+def Lambda.toString : Λ' → String
   | bvar n => s!"°{n.repr}"
   | fvar n => n.repr
   | abs e => s!"λ {e.toString}"
@@ -21,31 +21,31 @@ def Lambda.toString : Λ → String
     | abs _, _ => s!"(({e₁.toString}) {e₂.toString})"
     | _, _ => s!"({e₁.toString} {e₂.toString})"
 
-instance : ToString Λ := ⟨Lambda.toString⟩
+instance : ToString Λ' := ⟨Lambda.toString⟩
 
-instance : Repr Λ where
+instance : Repr Λ' where
   reprPrec M _ := M.toString.toFormat
 
-instance : Coe Nat Λ := ⟨λ n => Lambda.fvar n⟩
+instance : Coe Nat Λ' := ⟨λ n => Lambda.fvar n⟩
 
 instance (n : Nat) : OfNat Lambda n := ⟨Lambda.fvar n⟩
 
 namespace Lambda
 
 @[simp]
-def fv : Λ → Finset ℕ
+def fv : Λ' → Finset ℕ
 | bvar _ => ∅
 | fvar x => {x}
 | app N₁ N₂ => (fv N₁) ∪ (fv N₂)
 | abs N => fv N
 
 @[simp]
-def fresh (x : ℕ) (N : Λ) := x ∉ fv N
+def fresh (x : ℕ) (N : Λ') := x ∉ fv N
 
 notation x "♯" N => fresh x N
 
 @[simp]
-def subst (v : Λ) (x : ℕ) (e : Λ) :=
+def subst (v : Λ') (x : ℕ) (e : Λ') :=
   match v with
   | bvar n    => °n
   | fvar y    => if x = y then e else y
@@ -54,8 +54,12 @@ def subst (v : Λ) (x : ℕ) (e : Λ) :=
 
 notation t "[" x " := " s "]" => subst t x s
 
+/--
+  Open term `v` at index `k` with term `u`.
+  That is, replace bound variable `°k` with term `u`.
+-/
 @[simp]
-def opening (v : Λ) (k : ℕ) (u : Λ) :=
+def opening (v : Λ') (k : ℕ) (u : Λ') :=
   match v with
   | bvar n => if n = k then u else °n
   | fvar y => y
@@ -69,47 +73,31 @@ def open₀ t u := t{0 ⇒ u}
 
 infixl:70 " ↑ " => open₀
 
+/--
+  Close term `v` at index `k` with variable `x`.
+  That is, replace free variable `x` with bound variable `°k`.
+-/
 @[simp]
-def closing (v : Λ) (k x : ℕ) : Lambda :=
+def closing (v : Λ') (k x : ℕ) : Λ' :=
   match v with
-  | bvar n    => °n
-  | fvar y    => if x = y then °k else y
+  | bvar n => °n
+  | fvar y => if x = y then °k else y
   | app N₁ N₂ => app (N₁.closing k x) (N₂.closing k x)
-  | abs N     => abs (N.closing (k + 1) x)
+  | abs N => λ (N.closing (k + 1) x)
 
-notation t "{" k " ⇐ "  x "}" => closing t k x
+notation t "{" k " ⇐ " x "}" => closing t k x
 
 @[simp]
 def close₀ t x := t{0 ⇐ x}
 
 infixl:70 " ↓ " => close₀
 
-end Lambda
-
-inductive Lc : Λ → Prop
-| lc_var {x : ℕ} : Lc x
-| lc_app {N₁ N₂} : Lc N₁ → Lc N₂ → Lc (N₁.app N₂)
-| lc_abs {N} :
-  ∀ L : Finset ℕ, (∀ x : ℕ, x ∉ L → Lc (N ↑ x)) → Lc (λ N)
-
 @[simp]
-def body (N : Λ) := ∃ (L : Finset ℕ), ∀ x, x ∉ L → Lc (N ↑ x)
+def unshift (N : Λ') (c d : ℕ) : Λ' :=
+  match N with
+  | bvar n => °n
+  | fvar x => if x < c then x else x - d
+  | app N₁ N₂ => (N₁.unshift c d).app (N₂.unshift c d)
+  | abs N => λ (N.unshift (c + 1) d)
 
-inductive Beta : Λ → Λ → Prop
-| basis {M N : Λ} : Beta ((λ M).app N) (M.open₀ N)
-| appr {M M' N : Λ}  : Beta M M' → Beta (M.app N) (M'.app N)
-| appl {M M' N : Λ} : Beta M M' → Beta (N.app M) (N.app M')
-| abs {M M' : Λ} : Beta M M' → Beta (λ M) (λ M')
-
-infixl:65 " →β " => Beta
-
-inductive BetaP : Λ → Λ → Prop
-| refl {M} : BetaP M M
-| abs {M M'} : BetaP M M' → BetaP (λ M) (λ M')
-| app {M M' N N'} : BetaP M M' → BetaP N N' → BetaP (M.app N) (M'.app N')
-| subst {M M' N N'} : BetaP M M' → BetaP N N' → BetaP ((λ M).app N) (M'.open₀ N')
-
-infixl:65 " ⇉ " => BetaP
-
-@[refl]
-theorem BetaP_rfl {M : Λ} : M ⇉ M := BetaP.refl
+end Lambda
