Lambda/LocalClosed.lean
@@ -1,0 +1,116 @@
+import Mathlib.Tactic
+import Lambda.Basic
+import Lambda.Properties
+
+open Lambda
+
+inductive Lc : Λ' → Prop
+| lc_var {x : ℕ} : Lc x
+| lc_app {N₁ N₂} : Lc N₁ → Lc N₂ → Lc (N₁.app N₂)
+| lc_abs (N) :
+  ∀ L : Finset ℕ, (∀ x ∉ L, Lc (N ↑ x)) → Lc (λ N)
+
+@[simp]
+def body (N : Λ') : Prop := ∃ L : Finset ℕ, ∀ x ∉ L, Lc (N ↑ x)
+
+namespace Lc
+
+lemma lc_abs_iff_body (N : Λ') : Lc (λ N) ↔ body N := by
+  constructor <;> simp_all
+  . intro h
+    cases h; expose_names; exists L
+  . intro L h
+    apply Lc.lc_abs
+    assumption
+
+@[simp]
+lemma open_rec_lc {M N : Λ'} {k : ℕ} : Lc M → M{k ⇒ N} = M := by
+  intro h
+  induction h generalizing k with
+  | lc_abs _ L h ih =>
+    simp_all
+    have ⟨x, hx⟩ := Infinite.exists_notMem_finset L
+    apply opening_lc_lemma
+    exact Ne.symm (Nat.zero_ne_add_one k)
+    apply ih
+    assumption
+  | _ => simp_all
+
+lemma subst_open {M N L : Λ'} {x k : ℕ} :
+  Lc L → M{k ⇒ N}[x := L] = M[x := L]{k ⇒ N[x := L]} := by
+  intro h
+  induction M generalizing k with
+  | bvar => simp; split; rfl; simp
+  | fvar => simp_all; split <;> simp_all
+  | _ => simp_all
+
+lemma subst_open_var {x y : ℕ} {N M : Λ'} :
+    Lc M → x ≠ y → (N[x := M]) ↑ y = (N ↑ y)[x := M] := by
+  intros
+  simp; rw [subst_open]
+  aesop; assumption
+
+section LcConservation
+
+variable {M N : Λ'}
+
+lemma opening_lc {N : Λ'} {k : ℕ} : Lc M → Lc (M{k ⇒ N}) := by aesop
+
+@[aesop safe]
+lemma open₀_lc {N : Λ'} : Lc M → Lc (M ↑ N) := by simp; aesop
+
+@[aesop safe]
+lemma app_lc : Lc M → Lc N → Lc (M.app N) := by
+  intro hm hn; apply lc_app <;> assumption
+
+lemma subst_lc {x : ℕ} : Lc M → Lc N → Lc (M[x := N]) := by
+  intro hm hn
+  induction hm with
+  | lc_var =>
+    simp; split; assumption; apply lc_var
+  | lc_app =>
+    simp; apply lc_app <;> aesop
+  | lc_abs M L h ih =>
+    simp [lc_abs_iff_body]
+    use L ∪ {x}
+    intro y hy
+    rw [← open₀, subst_open_var hn (by aesop)]
+    apply ih
+    aesop
+
+@[simp]
+lemma subst_as_close_open {x k z : ℕ} : Lc N → N{k ⇐ x}{k ⇒ z} = N[x := z] := by
+  intro hn
+  induction hn generalizing k with
+  | lc_var => simp; split <;> simp
+  | lc_app => simp_all
+  | lc_abs N L h ih =>
+    simp
+    have ⟨y, hy⟩ :=
+      let N₁ := N{k + 1 ⇐ x}{k + 1 ⇒ z}
+      let N₂ := N[x := z]
+      Infinite.exists_notMem_finset (L ∪ {x} ∪ N.fv ∪ N₁.fv ∪ N₂.fv)
+    simp at hy
+    have := @ih y hy.2.1 (k + 1)
+    rw [
+      open₀, ← open_close_var (by aesop) (by aesop) (by aesop),
+      ← open₀, ← open₀, ← subst_open_var lc_var (by aesop)
+    ] at this
+    apply @open₀_injective y <;> simp
+    . exact hy.2.2.2.1
+    . exact hy.2.2.2.2
+    exact this
+
+lemma abs_lc : Lc M → Lc (λ (M ↓ 0)) := by
+  intro h
+  apply lc_abs
+  intros
+  simp_all
+  apply subst_lc
+  assumption
+  exact lc_var
+  use {1}
+  aesop
+
+end LcConservation
+end Lc
