Lambda/Properties.lean
@@ -3,44 +3,57 @@ import Mathlib.Tactic
 
 open Lambda
 
-lemma exists_notFree_var (N : Λ) : ∃ x, x ♯ N := Infinite.exists_notMem_finset (fv N)
-
-lemma lc_abs_iff_body (N : Λ) : Lc (λ N) ↔ body N := by
-  constructor <;> simp_all
-  . intro h
-    cases h; expose_names; exists L
-  . intro L h
-    apply Lc.lc_abs
-    assumption
+lemma exists_notFree_var (N : Λ') : ∃ x, x ♯ N := Infinite.exists_notMem_finset (fv N)
 
 @[simp]
-lemma close_open {k x : ℕ} {N : Λ} : (x ♯ N) → N{k ⇒ x}{k ⇐ x} = N := by
-  intro h₁; simp at h₁
-  induction N generalizing k
-  case bvar => simp; split <;> simp; omega
-  all_goals (unfold fv at h₁; simp_all)
-
-lemma close_open_var {N : Λ} {x : ℕ} : (x ♯ N) → (N ↑ x) ↓ x = N := by exact close_open
-
-@[simp]
-lemma subst_fresh {N M : Λ} {x : ℕ} : (x ♯ N) → N[x := M] = N := by
+lemma subst_fresh {N M : Λ'} {x : ℕ} : (x ♯ N) → N[x := M] = N := by
   intro h₁; simp at h₁
   induction N <;> (unfold fv at h₁; simp_all)
 
-lemma subst_intro {N M : Λ} {x k : ℕ} : (x ♯ N) → N{k ⇒ M} = (N{k ⇒ x})[x := M] := by
+lemma subst_intro {N M : Λ'} {x k : ℕ} : (x ♯ N) → N{k ⇒ M} = (N{k ⇒ x})[x := M] := by
   intro h₁; simp at h₁
   induction N generalizing k
   case bvar => simp; split <;> simp
   all_goals unfold fv at h₁; simp_all
 
-theorem substitution {M N L : Λ} {x y : ℕ} (xny : x ≠ y) (xnfv : x ♯ L) :
+theorem substitution {M N L : Λ'} {x y : ℕ} (xny : x ≠ y) (xnfv : x ♯ L) :
   M[x := N][y := L] = M[y := L][x := N[y := L]] := by
   induction M
   case fvar => repeat (first | simp_all | split)
   all_goals simp_all
 
+lemma subst_opening {N M : Λ'} {k : ℕ} (x : ℕ) : (x ♯ N) → N{k ⇒ M} = N{k ⇒ x}[x := M] := by
+  intro h; simp at h
+  induction N generalizing k
+  case bvar => simp; split <;> simp
+  all_goals (unfold fv at h); aesop
+
+lemma subst_open₀ {N M : Λ'} {x : ℕ} : (x ♯ N) → N ↑ M = (N ↑ x)[x := M] := by
+  simp; apply subst_opening
+
+lemma notFree_open_conservation {N M : Λ'} {k : ℕ} (x : ℕ) :
+  (x ♯ M) → (x ♯ N) → (x ♯ M{k ⇒ N}) := by
+  induction M generalizing k <;> repeat (first | simp_all | split)
+
+lemma open_comm {x₁ x₂ y₁ y₂ : ℕ} {M : Λ'} :
+    x₁ ≠ x₂ → M{x₁ ⇒ y₁}{x₂ ⇒ y₂} = M{x₂ ⇒ y₂}{x₁ ⇒ y₁} := by
+  intro h
+  induction M generalizing x₁ x₂ with
+  | bvar n => repeat (first | simp_all | split)
+  | fvar => simp
+  | app => simp; constructor <;> aesop
+  | abs => simp; aesop
+
+lemma open_close_var {n m x y z : ℕ} {N : Λ'}:
+    n ≠ m → x ≠ y → (y ♯ N) → N{n ⇐ x}{n ⇒ z}{m ⇒ y} = N{m ⇒ y}{n ⇐ x}{n ⇒ z} := by
+  intro hnm hxy hy; simp at hy
+  induction N generalizing n m
+  -- The cases of bvar and fvar are followed by making cases on the equalities of n,m,x and y
+  -- The cases of app and abs are followed by simplificantion
+  all_goals repeat (first | simp_all | split)
+
 @[simp]
-lemma opening_lc_lemma {M N L : Λ} {i j : ℕ} :
+lemma opening_lc_lemma {M N L : Λ'} {i j : ℕ} :
   i ≠ j → M{j ⇒ N}{i ⇒ L} = M{j ⇒ N} → M{i ⇒ L} = M := by
   intro hij h₁
   induction M generalizing i j with
@@ -50,37 +63,20 @@ lemma opening_lc_lemma {M N L : Λ} {i j : ℕ} :
     simp_all; have ⟨h₁, h₂⟩ := h₁; constructor <;> aesop
   | abs => simp_all; aesop
 
+@[simp]
+lemma close_open {x k : ℕ} {N : Λ'} :
+    (x ♯ N) → N{k ⇒ x}{k ⇐ x} = N := by
+  intro hx; simp at hx
+  induction N generalizing k
+  all_goals repeat (first | simp_all | split)
 
 @[simp]
-lemma open_rec_lc {M N : Λ} {k : ℕ} : Lc M → M{k ⇒ N} = M := by
-  intro h
-  induction h generalizing k with
-  | lc_var => simp
-  | lc_app => simp_all
-  | lc_abs L _ ih  =>
-    simp_all
-    have ⟨x, hx⟩ : ∃ x, x ∉ L := Infinite.exists_notMem_finset L
-    apply opening_lc_lemma
-    exact Ne.symm (Nat.zero_ne_add_one k)
-    apply ih; assumption
+lemma close_open_var {x : ℕ} {N : Λ'} :
+  (x ♯ N) → (N ↑ x) ↓ x = N := by
+  intro hx; simp_all
 
-lemma subst_opening {N M : Λ} {k : ℕ} (x : ℕ) : (x ♯ N) → N{k ⇒ M} = N{k ⇒ x}[x := M] := by
-  intro h; simp at h
-  induction N generalizing k
-  case bvar => simp; split <;> simp
-  all_goals (unfold fv at h); aesop
-
-lemma subst_open₀ {N M : Λ} {x : ℕ} : (x ♯ N) → N ↑ M = (N ↑ x)[x := M] := by
-  simp; apply subst_opening
-
-lemma subst_open {M N L : Λ} {x k : ℕ} :
-  Lc L → M{k ⇒ N}[x := L] = M[x := L]{k ⇒ N[x := L]} := by
-  intro h
-  induction M generalizing k with
-  | bvar => simp; split; rfl; simp
-  | fvar => simp_all; split <;> simp_all
-  | _ => simp_all
-
-lemma notFree_open_conservation {N M : Λ} {k : ℕ} (x : ℕ) :
-  (x ♯ M) → (x ♯ N) → (x ♯ M{k ⇒ N}) := by
-  induction M generalizing k <;> repeat (first | simp_all | split)
+@[simp]
+lemma open₀_injective {x : ℕ} {N M : Λ'} :
+    (x ♯ N) → (x ♯ M) → (N ↑ x = M ↑ x) → N = M := by
+  intro hn hm h
+  rw [← @close_open_var x N hn, ← @close_open_var x M hm, h]
