Lambda/Reduction.lean
@@ -1,0 +1,6 @@
+import Mathlib.Tactic
+import Lambda.Basic
+import Lambda.LocalClosed
+
+open Lambda
+open Lc
