Lambda/WellDefined.lean
@@ -1,0 +1,45 @@
+import Lambda.Basic
+import Lambda.LocalClosed
+import Mathlib.Tactic
+
+open Lc
+open Lambda
+
+def LambdaLC := { N : Λ' // Lc N }
+
+abbrev Λ := LambdaLC
+
+def LambdaLC.toString : Λ → String := fun ⟨M, _⟩ => Lambda.toString M
+
+instance : ToString Λ := ⟨LambdaLC.toString⟩
+
+instance : Repr Λ where
+  reprPrec M _ := M.toString.toFormat
+
+instance : Coe Nat Λ := ⟨fun n => ⟨Lambda.fvar n, lc_var⟩⟩
+
+instance (n : Nat) : OfNat LambdaLC n := ⟨⟨Lambda.fvar n, lc_var⟩⟩
+
+namespace LambdaLC
+
+def app (N M : Λ) : Λ := ⟨N.1.app M.1, app_lc N.2 M.2⟩
+def abs (N : Λ) : Λ := ⟨λ (N.1 ↓ 0), abs_lc N.2⟩
+
+prefix:100 "λ " => LambdaLC.abs
+
+def subst (N : Λ) (x : ℕ) (M : Λ) : Λ := ⟨N.1[x := M.1], subst_lc N.2 M.2⟩
+
+notation t "[" x " := " s "]" => LambdaLC.subst t x s
+
+end LambdaLC
+
+open LambdaLC
+
+def x : Λ := 0
+def y : Λ := 1
+def z : Λ := 2
+
+def L : Λ := (λ y.app (x.app x))[1 := 0]
+def Y : Λ := λ (L.app L)
+
+#eval Y
